Added stuff

examples/fac_master/tzwrap/fa2/multi_asset/FA2_Multi_Asset.v
@@ -73,8 +73,8 @@ Definition fa2_init (chain : Chain) (ctx: ContractCallContext) (setup: Setup) : 
     let tokens := setup.(tokens) in
     let meta_data_uri := setup.(meta_data_uri) in
     let meta := FMap.update EmptyString (Some meta_data_uri) FMap.empty in
-    let token_metadata := fold_right (fun (token_metadata : TokenMetadata) (acc : TokenMetaDataStorage) => FMap.update token_metadata.(tm_token_id) (Some token_metadata) acc) FMap.empty tokens in
-    let supply := fold_right (fun (token_metadata : TokenMetadata) (acc : TokenTotalSupply) => FMap.update token_metadata.(tm_token_id) (Some 0) acc) FMap.empty tokens in
+    let token_metadata := fold_left (fun (acc : TokenMetaDataStorage) (token_metadata : TokenMetadata) => FMap.update token_metadata.(tm_token_id) (Some token_metadata) acc) tokens FMap.empty in
+    let supply := fold_left (fun (acc : TokenTotalSupply) (token_metadata : TokenMetadata) => FMap.update token_metadata.(tm_token_id) (Some 0) acc) tokens FMap.empty in
     Some ({|
         fa2_admin := {|
             tas_admin := admin ;
@@ -344,15 +344,15 @@ Qed.
 
 (**----------------- FA2_Multi_Asset -----------------**)
 Definition sum_tx (txs : list MintBurnTx) (id : token_id): Z :=
-    fold_right 
-    (fun (tx : MintBurnTx) (acc : Z) => 
+    fold_left 
+    (fun (acc : Z) (tx : MintBurnTx) => 
         (
             if tx.(mint_burn_token_id) =? id
             then (acc + (Z.of_N tx.(mint_burn_amount)))%Z
             else 0%Z
         )
         )
-    0%Z txs.
+    txs 0%Z.
 
 Definition mint_or_burn (id : token_id) (msg : option MultiAssetParam) : Z :=
     match msg with
@@ -368,16 +368,50 @@ Definition mint_or_burn (id : token_id) (msg : option MultiAssetParam) : Z :=
     | _ => 0
     end.
 
+Lemma not_or_is_and {p1 p2} :
+    ~ (p1 \/ p2) -> ~p1 /\ ~p2.
+Proof.
+    intros. easy. 
+Qed.
+
+Lemma NoDup_map_cons {A B : Type} {f: A -> B} {l a} :
+    NoDup (map f (a :: l)) -> NoDup (map f l).
+Proof.
+    intros. cbn in H. rewrite NoDup_cons_iff in H. inversion H. easy.
+Qed.
+
+Lemma init_total_supply_fold_find_add {tm_token_id a l m} :
+    NoDup (a.(tm_token_id) :: (map (fun x => x.(tm_token_id)) l)) ->
+    (fold_left 
+        (fun (acc : TokenTotalSupply) (token_metadata : TokenMetadata) => 
+            FMap.add token_metadata.(tm_token_id) 0 acc) 
+            l (FMap.add a.(tm_token_id) 0 m)) =
+    FMap.add a.(tm_token_id) 0 ((fold_left 
+    (fun (acc : TokenTotalSupply) (token_metadata : TokenMetadata) => 
+        FMap.add token_metadata.(tm_token_id) 0 acc) 
+        l m)).
+Proof.
+    intros. generalize dependent m. induction l.
+    - easy.
+    - intros. cbn. rewrite NoDup_cons_iff in H. inversion H. cbn in H0. 
+    apply not_or_is_and in H0. inversion H0. intros. setoid_rewrite FMap.add_commute; try easy.
+    apply IHl. rewrite NoDup_cons_iff. split; try easy. inversion H.
+    apply NoDup_map_cons in H5. easy.
+Qed.
+
 Lemma init_total_supply_correct {chain ctx setup state fa2_token_id total_supply} :
+    NoDup ((map (fun x => x.(tm_token_id)) setup.(tokens))) ->
     FMap.find fa2_token_id state.(fa2_assets).(token_total_supply) = Some total_supply ->
     fa2_init chain ctx setup = Some state ->
     total_supply = 0.
 Proof.
     intros. contract_simpl fa2_receive fa2_init. induction tokens.
-    - cbn in H. setoid_rewrite FMap.find_empty in H. inversion H.
+    - cbn in H0. setoid_rewrite FMap.find_empty in H0. inversion H0.
     - cbn in *. destruct (fa2_token_id =? (tm_token_id a)) eqn:E.
-        + rewrite N.eqb_eq in E. rewrite E in H. setoid_rewrite FMap.find_add in H. inversion H. reflexivity.
-        + rewrite N.eqb_neq in E. setoid_rewrite FMap.find_add_ne in H; try easy.
+        + rewrite N.eqb_eq in E. rewrite E in H0. rewrite init_total_supply_fold_find_add in H0; try easy.
+          setoid_rewrite FMap.find_add in H0. inversion H0. reflexivity.
+        + rewrite N.eqb_neq in E. rewrite init_total_supply_fold_find_add in H0; try easy.
+          setoid_rewrite FMap.find_add_ne in H0;try easy. apply IHl in H0; try easy. apply NoDup_map_cons in H. easy.
 Qed.
 
 
@@ -406,11 +440,13 @@ Lemma assets_endpoint_preserves_total_supply {prev_state next_state acts chain c
     fa2_receive chain ctx prev_state (Some (Assets param)) = Some (next_state, acts) ->
     prev_state.(fa2_assets).(token_total_supply) = next_state.(fa2_assets).(token_total_supply).
 Proof.
-    intros. contract_simpl fa2_receive fa2_init. destruct param.
-    - inversion H1. destruct (transfer ctx transfers default_operator_validator (fa2_assets prev_state)) in H2.
+    intros. contract_simpl fa2_receive fa2_init. cbn. destruct param.
+    - inversion H1. destruct (transfer ctx transfers default_operator_validator (fa2_assets prev_state)) in H2;
      now inversion H2.
-
-Qed. 
+    - inversion H1. destruct (get_balance balanceOf (ledger (fa2_assets prev_state))
+    (token_metadata (fa2_assets prev_state))); try easy.
+    - inversion H1. destruct (fa2_update_operators ctx updates (operators (fa2_assets prev_state))); try easy.
+Qed.        
 
 Lemma set_admin_preserves_total_supply {prev_state next_state acts chain ctx addr} :
     fa2_receive chain ctx prev_state (Some (Admin (Token_admin (Set_admin addr)))) = Some (next_state, acts) ->
@@ -427,7 +463,7 @@ Proof.
     cbn. unfold fail_if_not_admin in H. destruct_address_eq; try easy.
 Qed. 
 
-Lemma fa2_correct : forall bstate caddr fa2_token_id total_supply (trace: ChainTrace empty_state bstate),
+(* Lemma fa2_correct : forall bstate caddr fa2_token_id total_supply (trace: ChainTrace empty_state bstate),
     env_contracts bstate caddr = Some (FA2_contract : WeakContract) ->
     exists cstate depinfo inc_calls,
         contract_state bstate caddr = Some cstate /\
@@ -451,5 +487,5 @@ Proof.
         + destruct param. destruct tokenAdmin.
             -- erewrite <- set_admin_preserves_total_supply in H; eauto. erewrite <- set_admin_does_not_change_minter; eauto.
             destruct_address_eq; now apply IH.
-            -- 
+            --  *)
 End FA2_Multi_Asset.
